theories/Vector.v
@@ -1,13 +1,13 @@
 Require Import Utils.
 
 Require Import Lia.
-
 Require Coq.Lists.List.
 Import List.ListNotations.
+Import Coq.NArith.BinNat.
 
 Record vector {A n} := {
   vector_list : list A;
-  vector_wf : length vector_list = n;
+  vector_wf : N.of_nat (length vector_list) = n;
 }.
 
 Arguments vector : clear implicits.
@@ -17,13 +17,13 @@ Register Build_vector as vcpu.vector.constructor.
 Register vector_list as vcpu.vector.list.
 Register vector_wf as vcpu.vector.wf.
 
-#[program] Definition vector_tail {A n} (v : vector A (S n)) : vector A n := {|
+#[program] Definition vector_tail {A n} (v : vector A (N.succ n)) : vector A n := {|
   vector_list := List.tl (vector_list v);
 |}.
 Next Obligation.
   intros A n v. specialize (vector_wf v) as H. destruct (vector_list v).
-  - simpl in H. congruence.
-  - simpl. simpl in H. injection H as H. auto.
+  - simpl in H. apply N.neq_0_succ in H. destruct H.
+  - simpl. simpl in H. lia.
 Qed.
 
 Notation bitvec := (vector bool).
@@ -34,8 +34,10 @@ Unset Program Cases.
   vector_list := List.map (fun '(b1, b2) => f b1 b2) (List.combine (vector_list bv1) (vector_list bv2));
 |}.
 Next Obligation.
-  intros f n bv1 bv2. rewrite List.map_length. rewrite List.combine_length. rewrite ? vector_wf.
-  apply PeanoNat.Nat.min_id.
+  intros f n bv1 bv2. rewrite List.map_length. rewrite List.combine_length.
+  rewrite <- (Nnat.Nat2N.id (length (vector_list bv1))).
+  rewrite <- (Nnat.Nat2N.id (length (vector_list bv2))).
+  rewrite ? vector_wf. rewrite PeanoNat.Nat.min_id. lia.
 Qed.
 
 Set Program Cases.
